puar/Useful.v
@@ -114,3 +114,129 @@ Proof.
   induction e; simpl in *; auto.
 Qed.
 
+
+Section rmNone.
+  Variable A: Type.
+
+  Definition indexIn i (ls: list A) :=
+    match Coq.Arith.Peano_dec.eq_nat_dec i (length ls) with
+    | left _ => ConstBool true
+    | right _ => ConstBool false
+    end.
+
+  Definition notNil (ls: list A) :=
+    match ls with
+    | nil => ConstBool false
+    | _ => ConstBool true
+    end.
+
+  Fixpoint rmNone (ls: list (option A)) :=
+    match ls with
+    | nil => nil
+    | Some x :: xs => x :: rmNone xs
+    | None :: xs => rmNone xs
+    end.
+
+  Fixpoint partition B n (ls: list B) :=
+    match n with
+    | 0 => match ls with
+           | nil => (nil, nil)
+           | x :: xs => (x :: nil, xs)
+           end
+    | S m => match ls with
+             | nil => (nil, nil)
+             | x :: xs =>
+               (x :: fst (partition m xs), snd (partition m xs))
+             end
+    end.
+
+  Lemma rmNonePartition: forall n (ls: list (option A)),
+      rmNone ls = rmNone (fst (partition n ls)) ++ rmNone (snd (partition n ls)).
+  Proof.
+    induction n; destruct ls; simpl; auto.
+    - destruct o; reflexivity.
+    - destruct o; simpl; f_equal; auto.
+  Qed.
+End rmNone.
+
+(* Fixpoint rmNone A (ls: list (option A)) := *)
+(*   match ls with *)
+(*   | nil => nil *)
+(*   | x :: xs => match x with *)
+(*                | Some y => [y] *)
+(*                | None => nil *)
+(*                end ++ rmNone xs *)
+(*   end. *)
+
+Definition countTrue (ls: list bool) := count_occ bool_dec ls true.
+
+Open Scope nat.
+Lemma countTrueLtSize ls: countTrue ls <= length ls.
+Proof.
+  induction ls; intros; unfold countTrue in *;
+    simpl; try match goal with
+               | |- context[match ?p with _ => _ end] =>
+                 destruct p
+               end; try Omega.omega.
+Qed.
+Close Scope nat.
+
+
+
+Require Import Kami.SymEvalTac Kami.SymEval Kami.MapReifyEx.
+
+Local Ltac simplMapUpds' t m k :=
+  let mr := mapVR_Others t O m in
+  rewrite <- (findMVR_find_string mr k eq_refl) in *;
+  cbn [findMVR_string] in *;
+  rewrite ?StringEq.string_eq_dec_false by (intro; discriminate).
+
+Ltac simplMapUpds :=
+  match goal with
+  | |- context[M.find (elt := sigT ?t) ?k ?m] =>
+    simplMapUpds' t m k
+  | H: context[M.find (elt := sigT ?t) ?k ?m] |- _ =>
+    simplMapUpds' t m k
+  end.
+
+Ltac SymEvalSimpl :=
+  SymEval';
+  cbv [SymSemAction semExpr or_wrap and_wrap eq_rect];
+  repeat (simplMapUpds; intros);
+  rewrite ?evalExprRewrite.
+
+Ltac substFind :=
+  match goal with
+  | H: (?y === ?n .[?s])%fmap , H': (?v === ?n .[ ?s])%fmap |- _ =>
+    rewrite H in H';
+    apply invSome in H';
+    apply Eqdep.EqdepTheory.inj_pair2 in H'; rewrite <- ?H' in *; clear H' v; intros
+  end.
+
+Lemma evalExprVarRewrite: forall k e, evalExpr (Var type k e) = e.
+Proof.
+  intros; reflexivity.
+Qed.
+
+Ltac initProcRight m r :=
+  simplInv; right;
+  exists ltac:(getRule m r);
+  split; [cbv [In getRules m]; auto|
+          unfold attrType at 1;
+          match goal with
+          | H: _ ?si ?ss |- _ =>
+            match type of si with
+            | RegsT => match type of ss with
+                       | RegsT => destruct H
+                       end
+            end
+          end;
+          SymEvalSimpl;
+          repeat substFind;
+          subst;
+          eexists; split;
+          [repeat econstructor; try (reflexivity || eassumption)|
+           rewrite ?evalExprVarRewrite;
+           esplit; simplMapUpds; try (reflexivity || eassumption)]
+         ].
+
